vale/code/arch/x64/interop/new/X64.MemoryAdapters.fst
@@ -1,0 +1,21 @@
+module X64.MemoryAdapters
+
+open Interop.Base
+module B = LowStar.Buffer
+module BS = X64.Bytes_Semantics_s
+module BV = LowStar.BufferView
+module HS = FStar.HyperStack
+module ME = X64.Memory
+module IB = Interop.Base
+module VS = X64.Vale.State
+friend X64.Memory
+module T = FStar.Tactics
+let buffer_eq = assert (ME.buffer == IB.buf_t) by (T.norm [delta_only [`%ME.buffer]]; T.trefl())
+let mem_eq = ()
+let buffer_addr_is_nat64 (#t:_) (x:ME.buffer t) (s:VS.state) = ()
+
+module V = X64.Vale.Decls
+module TS = X64.Taint_Semantics_s
+friend X64.Vale.Decls
+
+let code_equiv : squash (V.va_code == TS.tainted_code) = ()
