vale/code/arch/x64/interop/new/X64.MemoryAdapters.fsti
@@ -7,15 +7,36 @@ module BV = LowStar.BufferView
 module HS = FStar.HyperStack
 module ME = X64.Memory
 module IB = Interop.Base
+module VS = X64.Vale.State
+module V = X64.Vale.Decls
+module TS = X64.Taint_Semantics_s
 
 val buffer_eq : squash (ME.buffer == IB.buf_t)
+
 unfold
-let as_vale_buffer (#t:_) (i:IB.buf_t t) : ME.buffer t = IB.coerce i
+let as_vale_buffer (#t:_) (i:IB.buf_t t)
+  : ME.buffer t
+  = IB.coerce i
+
 unfold
-let as_lowstar_buffer (#t:_) (i:ME.buffer t) : IB.buf_t t = IB.coerce i
+let as_lowstar_buffer (#t:_) (i:ME.buffer t)
+  : IB.buf_t t
+  = IB.coerce i
 
 val mem_eq : squash (ME.mem == IB.mem)
+
 unfold
-let as_mem (m:ME.mem) : IB.mem = IB.coerce m
+let as_mem (m:ME.mem)
+  : IB.mem
+  = IB.coerce m
+
 unfold
-let as_vale_mem (m:IB.mem) : ME.mem = IB.coerce m
+let as_vale_mem (m:IB.mem)
+  : ME.mem
+  = IB.coerce m
+
+val buffer_addr_is_nat64 (#t:_) (x:ME.buffer t) (s:VS.state)
+  : Lemma (0 <= ME.buffer_addr x VS.(s.mem) /\
+           ME.buffer_addr x VS.(s.mem) < pow2 64)
+
+val code_equiv : squash (V.va_code == TS.tainted_code)
